LeanCats/Lemmas.lean
@@ -1,0 +1,404 @@
+import LeanCats.HerdingCats
+
+open Primitives
+
+lemma tc_step_N_swap
+  (n : Nat)
+  (input : List Event)
+  (tc : List (Event × Event)) :
+  tc_step_N n input (tc_step input tc) = tc_step input (tc_step_N n input tc) :=
+  by
+    induction n generalizing tc with
+    | zero => {
+      aesop
+    }
+    | succ n' h' => {
+      rw [tc_step_N]
+      rw [tc_step_N]
+      rw [h' (tc_step input tc)]
+    }
+
+lemma tc_step_N_add (input : List Event) (m n : Nat) (tc : List (Event × Event)) :
+  tc_step_N (m + n) input tc = tc_step_N n input (tc_step_N m input tc) := by
+  induction m generalizing n with
+  | zero =>
+    simp [tc_step_N]
+  | succ m' ih =>
+    repeat rw [tc_step_N]
+    have h : tc_step_N (m' + n + 1) input tc = tc_step_N (n + 1) input (tc_step_N m' input tc) :=
+      by
+        apply ih (n + 1)
+    nth_rewrite 2 [tc_step_N] at h
+    rw [Nat.add_assoc]
+    nth_rewrite 2 [Nat.add_comm]
+    rw [<-Nat.add_assoc]
+    rw [h]
+    nth_rewrite 2 [tc_step_N_swap]
+    rfl
+
+lemma tc_base_is_tc
+  {a b : Event}
+  (r : Event -> Event -> Prop)
+  (elems : List Event)
+  [DecidableRel r]
+  : (a, b) ∈ tc_base r elems -> Relation.TransGen r a b :=
+  by
+    intro h
+    simp_all
+    have rab : r a b :=
+      by
+        aesop
+    apply Relation.TransGen.single
+    exact rab
+
+lemma tc_step_contains_prev_step
+  (input : List Event)
+  {a b : Event}
+  (tc : List (Event × Event))
+  : (a, b) ∈ tc_step input tc -> (a, b) ∈ tc_step input (tc_step input tc) :=
+  by
+    aesop
+
+lemma tc_N_succ_steps_includes_N_succ
+  (input : List Event)
+  (n : Nat)
+  (tc : List (Event × Event))
+  : tc_step_N n input tc ⊆ tc_step_N (n+1) input tc :=
+    by
+      intro h
+      induction n with
+      | zero => {
+        aesop
+      }
+      | succ n' h' => {
+        intro h''
+        unfold tc_step_N
+        unfold tc_step_N
+        rw [tc_step_N_swap]
+        rw [tc_step_N_swap]
+        apply tc_step_contains_prev_step
+        unfold tc_step_N at h''
+        rw [tc_step_N_swap] at h''
+        exact h''
+      }
+
+-- This is the tail definition of the TransGen.
+lemma tc_step_trans
+  {a b c: Event}
+  (input : List Event)
+  (r : Event -> Event -> Prop)
+  [DecidableRel r]
+  (h₁ : (a, b) ∈ tc_base r input)
+  (h₂ : (b, c) ∈ tc_base r input) :
+  (a, c) ∈ tc_step input (tc_base r input) :=
+  by
+    simp
+    apply Or.inl
+    aesop
+
+lemma tc_step_tranGen
+  {a b: Event}
+  (input : List Event)
+  {r : Event -> Event -> Prop}
+  [DecidableRel r]
+  {ha : a ∈ input}
+  {hb : b ∈ input}
+  {tc : List (Event × Event)}
+  (hab : (a, b) ∈ tc_step input (tc))
+  (htrans : ∀a b, (a, b) ∈ tc -> Relation.TransGen r a b) :
+  Relation.TransGen r a b :=
+  by
+    aesop
+    have transaw : Relation.TransGen r a w :=
+    by
+      apply (htrans a w) left
+
+    have transwb : Relation.TransGen r w b :=
+    by
+      apply (htrans w b) right
+
+    apply Relation.TransGen.trans transaw transwb
+
+lemma tc_step_trans'
+  {a b c: Event}
+  (input : List Event)
+  {ha : a ∈ input}
+  {hb : b ∈ input}
+  {hc : c ∈ input}
+  {tc : List (Event × Event)}
+  (h₁ : (a, b) ∈ tc)
+  (h₂ : (b, c) ∈ tc) :
+  (a, c) ∈ tc_step input (tc) :=
+  by
+    induction tc with
+    | nil => {
+      aesop
+    }
+    | cons head tail tail_ih => {
+      aesop
+    }
+
+lemma tc_step_N_trans
+  {n : Nat}
+  {a b c: Event}
+  (input : List Event)
+  {ha : a ∈ input}
+  {hb : b ∈ input}
+  {hc : c ∈ input}
+  (r : Event -> Event -> Prop)
+  [DecidableRel r]
+  (h₁ : (a, b) ∈ tc_step_N n input (tc_base r input))
+  (h₂ : (b, c) ∈ tc_step_N n input (tc_base r input)) :
+  (a, c) ∈ tc_step_N (n+1) input (tc_base r input) :=
+  by
+    unfold tc_step_N
+    rw [tc_step_N_swap]
+    apply tc_step_trans'
+    exact ha
+    exact hb
+    exact hc
+    exact h₁
+    exact h₂
+
+lemma tc_N_steps_in_tc_N_succ'
+  {a b : Event}
+  (n : Nat)
+  (r : Event -> Event -> Prop)
+  [DecidableRel r]
+  (input : List Event)
+  : (a, b) ∈ tc_step_N n input (tc_base r input) -> (a, b) ∈ tc_step_N (n+1) input (tc_base r input) :=
+    by
+      intro h
+      induction n with
+      | zero => {
+        aesop
+      }
+      | succ n' ih => {
+        apply tc_N_succ_steps_includes_N_succ
+        apply h
+      }
+
+lemma tc_step_base_transGen
+  {a b: Event}
+  (input : List Event)
+  {ha : a ∈ input}
+  {hb : b ∈ input}
+  {r : Event -> Event -> Prop}
+  [DecidableRel r]
+  (h : (a, b) ∈ tc_step input (tc_base r input)) :
+  Relation.TransGen r a b :=
+  by
+    simp_all
+    aesop
+    {
+      have hawTrans : Relation.TransGen r a w :=
+      by
+        apply Relation.TransGen.single
+        exact right_1
+
+      have hwbTrans : Relation.TransGen r w b :=
+      by
+        apply Relation.TransGen.single
+        exact right
+
+      apply Relation.TransGen.trans hawTrans hwbTrans
+    }
+    {
+      apply Relation.TransGen.single
+      exact h_2
+    }
+
+lemma TransGen_tc_step
+  {a b c: Event}
+  (input : List Event)
+  {ha : a ∈ input}
+  {hc : c ∈ input}
+  {r : Event -> Event -> Prop}
+  [DecidableRel r]
+  (tc : List (Event × Event))
+  (habi : (a, b) ∈ tc)
+  (hbci : (b, c) ∈ tc) :
+  (a, c) ∈ tc_step input tc :=
+  by
+    aesop
+
+lemma tc_N_steps_is_tc
+  {a b: Event}
+  (n : Nat)
+  (r : Event -> Event -> Prop)
+  [DecidableRel r]
+  (input : List Event)
+  {ha : a ∈ input}
+  {hb : b ∈ input}
+  {tc : List (Event × Event)}
+  (htrans : ∀ a b, (a, b) ∈ tc -> Relation.TransGen r a b)
+  : (a, b) ∈ tc_step_N n input tc -> Relation.TransGen r a b := by
+    intro h'
+    induction n generalizing tc with
+    | zero => {
+      unfold tc_step_N at h'
+      apply htrans
+      exact h'
+    }
+    | succ n' h'' => {
+      sorry
+    }
+
+lemma comp_tc_towards_tc
+  {a b : Event}
+  {r : Event -> Event -> Prop}
+  [DecidableRel r]
+  (input : List Event) :
+  a ∈ input
+  -> b ∈ input
+  -> (a, b) ∈ comp_tc input r
+  -> Relation.TransGen r a b := by
+    intro ha hb
+    unfold comp_tc
+    intro h
+    apply tc_N_steps_is_tc
+    exact ha
+    exact hb
+    have hbase : ∀ (a b : Event), (a, b) ∈ (tc_base r input) → Relation.TransGen r a b :=
+    by
+      intro a b
+      intro h'
+      simp at h'
+      apply And.right at h'
+      apply Relation.TransGen.single
+      exact h'
+
+    exact hbase
+    exact h
+
+lemma tc_base_in_product
+  (r : Event -> Event -> Prop)
+  [DecidableRel r]
+  (input : List Event) :
+  tc_base r input ⊆ input.product input :=
+  by
+    aesop
+
+lemma tc_step_in_product
+  (r : Event -> Event -> Prop)
+  [DecidableRel r]
+  (input : List Event) :
+  tc_step input (tc_base r input) ⊆ input.product input :=
+  by
+    aesop
+
+lemma tc_step_N_in_product
+  (n : Nat)
+  (input : List Event)
+  (tc : List (Event × Event))
+  (h : tc ⊆ input.product input) :
+  tc_step_N n input tc ⊆ input.product input :=
+  by
+    induction n with
+    | zero => {
+      simp
+      exact h
+    }
+    | succ n' ih => {
+      unfold tc_step_N
+      rw [tc_step_N_swap]
+      aesop
+    }
+
+-- Every pairs are connected (transitive)
+-- This states that the product contains all the possible results.
+-- lemma tc_comp_upper_bound
+--   {a b : Event}
+--   (r : Event -> Event -> Prop)
+--   [DecidableRel r]
+--   (input : List Event)
+--   (ha : a ∈ input)
+--   (hb : b ∈ input) :
+--   (comp_tc input r) ⊆ input.product input :=
+--   by
+--     intro p hcomp
+--     unfold comp_tc at hcomp
+--     apply (tc_step_N_in_product r (input.length * input.length) input)
+--     exact hcomp
+
+
+-- We want to calcualte the maximum or minimum pairs we can add for each round.
+-- We need to specify the mimimum rounds that can make sure we can find all the pairs.
+-- Suppose we only filter out one pair in each round, then we need at least (tc.product tc).length to get all the pairs.
+-- 1. First we need to make sure that the input.product input is the upper bound, we can't find any more pair that is out of this bound.
+
+-- Every pairs are connected (transitive)
+-- This states that the product contains all the possible results.
+lemma tc_comp_upper_bound
+  {r : Event -> Event -> Prop}
+  [DecidableRel r]
+  (input : List Event) :
+  (comp_tc input r) ⊆ input.product input :=
+  by
+    unfold comp_tc
+    apply tc_step_N_in_product
+    aesop
+
+
+-- We need to prove, after some iterations the (a, b) won't be changed
+-- The computation is limited by input, so the input.product input is what we can calcuate at most.
+-- a ∧ b ∈ input means the all possible results are combinations of (a, b)
+lemma tc_towards_comp_tc
+  {a b : Event}
+  (r : Event -> Event -> Prop)
+  [DecidableRel r]
+  (input : List Event) :
+  a ∈ input
+  -> b ∈ input
+  -> Relation.TransGen r a b
+  -> (a, b) ∈ comp_tc input r :=
+  by
+    intro ha
+    intro hb
+    intro htrans
+    unfold comp_tc
+    induction htrans with
+    | single hrel => {
+      -- TODO(Zhiyang): Every pair in tc_comp is r a b
+      sorry
+    }
+    | tail htrans hrel ih => {
+      sorry
+    }
+
+theorem tc_comp_is_tc
+  {a b : Event}
+  (r : Event -> Event -> Prop)
+  [DecidableRel r]
+  (input : List Event)
+  (ha : a ∈ input)
+  (hb : b ∈ input) :
+  Relation.TransGen r a b <-> (a, b) ∈ comp_tc input r :=
+  by
+    apply Iff.intro
+    {
+      intro htrans
+      apply tc_towards_comp_tc
+      {
+        exact ha
+      }
+      {
+        exact hb
+      }
+      {
+        exact htrans
+      }
+    }
+    {
+      intro hcomp
+      apply comp_tc_towards_tc
+      {
+        exact ha
+      }
+      {
+        exact hb
+      }
+      {
+        exact hcomp
+      }
+    }
