LeanCats/LitmusParser.lean
@@ -1,0 +1,71 @@
+import LeanCats.AST
+import LeanCats.HerdingCats
+
+namespace LitmusParser
+
+def ins2event
+  (t_id : Nat)
+  (thread : Primitives.Thread)
+  (ins : LitmusAST.Instruction)
+  (id : String) : Primitives.Event :=
+  {
+    id := id
+    t_id := t_id
+    t := thread
+    ln := ins.line_num
+    a := ins.action
+  }
+
+def prog2events (prog : LitmusAST.Program) (start_id : Nat) : List Primitives.Event × Nat :=
+  let thread : Primitives.Thread := Primitives.Thread.mk prog.thread
+  let ins2event := ins2event prog.thread thread
+
+  let rec process_instructions (instructions : List LitmusAST.Instruction) (curr_id : Nat) : List Primitives.Event × Nat :=
+    match instructions with
+    | [] => ([], curr_id)
+    | ins :: rest =>
+      let id_str := toString curr_id
+      let event := ins2event ins id_str
+      let (rest_events, next_id) := process_instructions rest (curr_id + 1)
+      (event :: rest_events, next_id)
+
+  process_instructions prog.instructions start_id
+
+def zip_instructions (insts : List Primitives.Event) : Set (Primitives.Event × Primitives.Event) :=
+  -- [r₁ r₂ r₂] -> [r₁ r₂] [r₂ r₃] -> [(r₁, r₂), (r₂, r₃)]
+  -- edge caes: return []
+  let insts₁ := insts.eraseIdx 0
+  let insts₂ := insts.dropLast
+
+  let insts := insts₁.zip insts₂
+
+  -- accumulate all the relations.
+  insts.foldl Primitives.R.add Primitives.R.empty
+
+def get_po (litmus : LitmusAST.Litmus) : Primitives.Relation :=
+  let start : Nat := 0
+
+  let rec process_programs (program : List LitmusAST.Program) (curr_id : Nat) : List (List Primitives.Event) × Nat :=
+    match program with
+    | [] => ([], curr_id)
+    | prog :: rest =>
+      let (prog_events, next_id) := prog2events prog curr_id
+      let (rest_programs_events, final_id) := process_programs rest next_id
+      (prog_events :: rest_programs_events, final_id)
+
+  let (all_program_events, _) := process_programs litmus.programs start
+
+  let events_list := all_program_events.map zip_instructions
+
+  events_list.foldl Set.union Primitives.R.empty
+
+def get_rf (litmus : LitmusAST.Litmus) : Primitives.Relation :=
+  sorry
+
+def get_fr (litmus : LitmusAST.Litmus) : Primitives.Relation :=
+  sorry
+
+-- There are lots of algorithms to find the read-from relation, like use-def chains (worklist to find)
+-- But for the sake of simplicity, we just use brute-force O(N!).
+
+end LitmusParser
